irritating situation about specificity of example.... should be easier in the general case.

plugins/vdm2isa/src/main/resources/RecursiveSet.thy
@@ -2,6 +2,8 @@ theory RecursiveSet
   imports VDMToolkit
 begin
 
+section \<open>Partial recursive functions\<close>
+
 function findzero :: "(nat \<Rightarrow> nat) \<Rightarrow> nat \<Rightarrow> nat"
 where
 "findzero f n = (if f n = 0 then n else findzero f (Suc n))"
@@ -15,6 +17,85 @@ where
 "findzero' f n = (if f n = 0 then n else findzero' f (Suc n))"
   by pat_completeness auto
 
+section \<open>Well foundedness study on bounded @{text nat_term}\<close>
+
+abbreviation \<open>NAT_MAX \<equiv> 3\<close>
+
+definition 
+  nat_term :: \<open>(\<nat> \<times> \<nat>) VDMSet\<close>
+  where
+  \<open>nat_term \<equiv> { (m, n) . n = Suc m \<and> n < NAT_MAX }\<close>
+
+lemma l_nat_term_eq: \<open>nat_term = { (0, 1), (1, 2) }\<close> (*, (2, 3), (3, 4) }\<close>*)
+  apply (simp add: nat_term_def, safe)
+  by (simp_all) 
+
+definition 
+  nat_fin_psub :: \<open>((\<nat> \<times> \<nat>) VDMSet \<times> (\<nat> \<times> \<nat>) VDMSet) VDMSet\<close>
+  where
+(*\<open>nat_fin_psub \<equiv> finite_psubset :: ((\<nat> \<times> \<nat>) VDMSet \<times> (\<nat> \<times> \<nat>) VDMSet) VDMSet\<close> *)
+  \<open>nat_fin_psub \<equiv> {(A, B). A \<subset> B \<and> finite B \<and> B \<subseteq> nat_term }\<close>
+
+lemma l_nat_fin_psub_eq1: \<open>{({(0, 1)}, {(0, 1), (1, 2)}), ({(1, 2)}, {(0, 1), (1, 2)}), ({}, {(0, 1), (1, 2)}), ({}, {(0, 1)}), ({}, {(1, 2)})} \<subseteq> nat_fin_psub\<close>  
+  apply (intro subsetI)
+  unfolding nat_fin_psub_def
+  apply (simp add: case_prod_beta)
+  apply (elim disjE, simp_all add: l_nat_term_eq)
+  by blast+
+
+lemma l_nat_fin_psub_eq2:\<open>nat_fin_psub \<subseteq> {({(0, 1)}, {(0, 1), (1, 2)}), ({(1, 2)}, {(0, 1), (1, 2)}), ({}, {(0, 1), (1, 2)}), ({}, {(0, 1)}), ({}, {(1, 2)})}\<close>
+  apply (intro subsetI)
+  unfolding nat_fin_psub_def
+  apply (simp add: case_prod_beta)
+  apply (elim conjE)
+  apply (simp add: subset_eq[of _ \<open>nat_term\<close>])
+  apply (rule disjI2)+
+  nitpick  
+  sorry 
+
+lemma \<open>nat_fin_psub = {({(0, 1)}, {(0, 1), (1, 2)}), ({(1, 2)}, {(0, 1), (1, 2)}), ({}, {(0, 1), (1, 2)}), ({}, {(0, 1)}), ({}, {(1, 2)})}\<close>
+  apply (rule equalityI)
+   apply (rule l_nat_fin_psub_eq2)
+  apply (rule l_nat_fin_psub_eq1)
+  done
+
+definition 
+  nat_lex_nat :: \<open>(((\<nat> \<times> \<nat>) set \<times> \<nat>) \<times> ((\<nat> \<times> \<nat>) set \<times> \<nat>)) set\<close>
+  where
+  \<open>nat_lex_nat \<equiv> nat_fin_psub <*lex*> nat_term\<close>
+
+definition lex_prod' :: "('a \<times>'a) set \<Rightarrow> ('b \<times> 'b) set \<Rightarrow> (('a \<times> 'b) \<times> ('a \<times> 'b)) set"
+    (infixr "<*lexi*>" 80)
+    where "ra <*lexi*> rb = {((a, b), (a', b')). (a, a') \<in> ra } \<union> 
+                            {((a, b), (a', b')). a = a' \<and> (b, b') \<in> rb}"
+
+lemma lex_prod_equiv: "(ra <*lex*> rb) = (ra <*lexi*>rb)"
+  by (safe, simp_all add: lex_prod_def lex_prod'_def)
+
+datatype T = A | B | C | D
+
+definition 
+  t_term :: \<open>(T \<times> T) VDMSet\<close>
+  where
+  \<open>t_term \<equiv> { (A, B), (B, C), (C, D) }\<close>
+
+definition 
+  t_fin_psub :: \<open>((T \<times> T) VDMSet \<times> (T \<times> T) VDMSet) VDMSet\<close>
+  where
+  \<open>t_fin_psub \<equiv> {(A, B). A \<subset> B \<and> finite B \<and> B \<subseteq> t_term }\<close>
+
+
+definition 
+  gen_lex_nat :: \<open>(('a VDMSet \<times> \<nat>) \<times> 'a VDMSet \<times> \<nat>) set\<close>
+  where
+  \<open>gen_lex_nat \<equiv> finite_psubset <*lex*> nat_term\<close>
+
+
+
+lemma \<open>nat_lex_nat = A\<close>
+  apply (simp add: nat_lex_nat_def nat_fin_psub_def nat_term_def lex_prod_def)
+  
+section \<open>Sum-set function\<close>
 
 definition 
   sumset_domain :: "VDMNat VDMSet \<Rightarrow> \<bool>" 
@@ -25,15 +106,42 @@ function (domintros)
   sumset :: "VDMNat VDMSet \<Rightarrow> VDMNat" 
   where 
   "sumset s = 
-    (if sumset_domain s then 
-        (if s = {} then 0 else let e = (SOME x . x \<in> s) in sumset (s - {e}) + e)
-     else 
-        undefined)"
+    (if s = {} then 0 else let e = (SOME x . x \<in> s) in sumset (s - {e}) + e)"
   by (blast, force)
 
 thm sumset.domintros
 thm sumset.pinduct
 
+lemma "x < y \<Longrightarrow> (x, y) \<in> less_than"
+  using less_than_def less_than_iff pred_nat_def by presburger
+
+definition 
+  sumset_term ::"(VDMNat VDMSet \<times> VDMNat VDMSet) set" where
+  "sumset_term \<equiv> { (s1, s2) . s1 \<subseteq> s2 \<and> finite s2 }"
+
+definition
+  sumset_lex :: "((\<nat> set \<times> (\<nat> \<times> \<nat>) set \<times> \<nat>) \<times> \<nat> set \<times> (\<nat> \<times> \<nat>) set \<times> \<nat>) set"
+  where
+  "sumset_lex \<equiv> (finite_psubset :: (nat VDMSet \<times> nat VDMSet) VDMSet)
+                 <*lex*> (finite_psubset :: ((nat \<times> nat) VDMSet \<times> (nat \<times> nat) VDMSet) VDMSet)
+                 <*lex*> pred_nat"
+
+lemma l1: "wf (finite_psubset :: (VDMNat VDMSet \<times> VDMNat VDMSet) VDMSet)" 
+  using wf_finite_psubset by blast
+
+lemma l2: "wf (finite_psubset :: ((VDMNat \<times> VDMNat) VDMSet \<times> (VDMNat \<times> VDMNat) VDMSet) VDMSet)"
+  using wf_finite_psubset by blast
+
+lemma l3: "wf ((finite_psubset :: (VDMNat VDMSet \<times> VDMNat VDMSet) VDMSet)
+               <*lex*> (finite_psubset :: ((VDMNat \<times> VDMNat) VDMSet \<times> (VDMNat \<times> VDMNat) VDMSet) VDMSet)
+               <*lex*> pred_nat)"
+  by (simp add: wf_lex_prod wf_pred_nat)
+  
+
+
+theorem sumset_termination:  
+  \<open>\<lbrakk>sumset_domain s\<rbrakk> \<Longrightarrow> sumset_dom s\<close>
+  thm wf_induct wf
 lemma lsum_set_domain_empty[simp]: "sumset_domain {}"
   unfolding sumset_domain_def 
   by simp
